Nemonuri/TransitionSystemLike/Interleaving.lean
@@ -26,9 +26,9 @@ class HasInterleaving (ts1: TransitionSystem.{us1, uact_l, uap_l}) (ts2: Transit
 --attribute [reducible, instance] HasInterleaving.act HasInterleaving.ap
 
 
-structure Interleaving (ts1: TransitionSystem.{us1, uact_l, uap_l}) (ts2: TransitionSystem.{us2, uact_l, uap_l}) (Act: Type uact_r) (AP: Type uap_r)  where
-  act: HasHUnion.Bundle ts1.Act ts2.Act Act
-  ap: HasHUnion.Bundle ts1.AP ts2.AP AP
+structure Interleaving (ts1: TransitionSystem.{us1, uact_l, uap_l}) (ts2: TransitionSystem.{us2, uact_l, uap_l}) where
+  act: HasHUnion.Bundle.{uact_l, uact_r} ts1.Act ts2.Act
+  ap: HasHUnion.Bundle.{uap_l, uap_r} ts1.AP ts2.AP
 
 
 --attribute [reducible, instance] Interleaving.actHasHUnionBundle Interleaving.apHasHUnionBundle
@@ -37,48 +37,48 @@ namespace Interleaving
 
 open HasHUnion
 
-variable {ts1: TransitionSystem.{us1, uact_l, uap_l}} {ts2: TransitionSystem.{us2, uact_l, uap_l}} {Act: Type uact_r} {AP: Type uap_r}
+variable {ts1: TransitionSystem.{us1, uact_l, uap_l}} {ts2: TransitionSystem.{us2, uact_l, uap_l}} --{Act: Type uact_r} {AP: Type uap_r}
 
 
 --abbrev inferAt (Act AP: Type _) [i: HasInterleaving ts1 ts2 Act AP] : HasInterleaving ts1 ts2 Act AP := i
 
-abbrev LeftActTypeAt (il: Interleaving ts1 ts2 Act AP) (lb: Label) : Type _ := il.act.hasHUnion.LeftTypeAt ts1.Act ts2.Act Act lb
+abbrev LeftActTypeAt (il: Interleaving ts1 ts2) (lb: Label) : Type _ := il.act.hasHUnion.LeftTypeAt ts1.Act ts2.Act lb
 
-def embedActAt (il: Interleaving ts1 ts2 Act AP) (lb: Label) (lv: il.LeftActTypeAt lb) : Act := il.act.hasHUnion.embedAt ts1.Act ts2.Act lb lv
+def embedActAt (il: Interleaving ts1 ts2) (lb: Label) (lv: il.LeftActTypeAt lb) : il.act.hasHUnion.R := il.act.hasHUnion.embedAt ts1.Act ts2.Act lb lv
 
 --def embedActAt (Act AP: Type _) [HasInterleaving ts1 ts2 Act AP] (lb: Label) (lv: LeftActTypeAt Act AP lb) : Act := il.toActHasHUnion.embedAt ts1.Act ts2.Act lb lv
 
 
 
 @[mk_iff]
-inductive Transition (il: Interleaving ts1 ts2 Act AP) : ts1.S → ts2.S → Act → ts1.S → ts2.S → Prop where
+inductive Transition (il: Interleaving ts1 ts2) : ts1.S → ts2.S → il.act.hasHUnion.R → ts1.S → ts2.S → Prop where
   | fst (s₁1: ts1.S) (a₁: ts1.Act) (s₁2: ts1.S) (req: s₁1 ─⌞a₁⌟→{ts1} s₁2) (s₂: ts2.S) : Transition il s₁1 s₂ (il.embedActAt .fst a₁) s₁2 s₂
   | snd (s₂1: ts2.S) (a₂: ts2.Act) (s₂2: ts2.S) (req: s₂1 ─⌞a₂⌟→{ts2} s₂2) (s₁: ts1.S) : Transition il s₁ s₂1 (il.embedActAt .snd a₂) s₁ s₂2
 
 @[reducible]
-def toTransitionSystem (il: Interleaving ts1 ts2 Act AP) : TransitionSystem where
+def toTransitionSystem (il: Interleaving ts1 ts2) : TransitionSystem where
   S := ts1.S × ts2.S
-  Act := letI := il.act.hasHUnion; HUnionElemAt ts1.Act ts2.Act Act
+  Act := letI := il.act.hasHUnion; HUnionElemAt ts1.Act ts2.Act
   I := Set.prod ts1.I ts2.I
-  AP := letI := il.ap.hasHUnion; HUnionElemAt ts1.AP ts2.AP AP
+  AP := letI := il.ap.hasHUnion; HUnionElemAt ts1.AP ts2.AP
   L s ap := letI := il.ap.memDecidable; il.ap.hasHUnion.hunionIndicator (ts1.labeling s.fst) (ts2.labeling s.snd) ap.val
   tr s1 a s2 := Transition il s1.fst s1.snd a s2.fst s2.snd
 
-def toTransitionSystemActAP (il: Interleaving ts1 ts2 Act AP) : TransitionSystem.OfActAP il.toTransitionSystem.Act il.toTransitionSystem.AP := il.toTransitionSystem.toActAP
+def toTransitionSystemActAP (il: Interleaving ts1 ts2) : TransitionSystem.OfActAP il.toTransitionSystem.Act il.toTransitionSystem.AP := il.toTransitionSystem.toActAP
 
 def inferAt
   (ts1: TransitionSystem.{us1, uact_l, uap_l}) (ts2: TransitionSystem.{us2, uact_l, uap_l})
-  (Act: Type uact_r) (AP: Type uap_r) [HasHUnion.Bundle ts1.Act ts2.Act Act] [HasHUnion.Bundle ts1.AP ts2.AP AP]
-  : Interleaving ts1 ts2 Act AP :=
+  [HasHUnion.Bundle ts1.Act ts2.Act] [HasHUnion.Bundle ts1.AP ts2.AP]
+  : Interleaving ts1 ts2 :=
   .mk inferInstance inferInstance
 
 end Interleaving
 
 def interleaveAt
-  (Act: Type uact_r) (AP: Type uap_r) (ts1: TransitionSystem.{us1, uact_l, uap_l}) (ts2: TransitionSystem.{us2, uact_l, uap_l})
-  [HasHUnion.Bundle ts1.Act ts2.Act Act] [HasHUnion.Bundle ts1.AP ts2.AP AP]
+  (ts1: TransitionSystem.{us1, uact_l, uap_l}) (ts2: TransitionSystem.{us2, uact_l, uap_l})
+  [HasHUnion.Bundle ts1.Act ts2.Act] [HasHUnion.Bundle ts1.AP ts2.AP]
   : TransitionSystem :=
-  (Interleaving.inferAt ts1 ts2 Act AP).toTransitionSystem
+  (Interleaving.inferAt ts1 ts2).toTransitionSystem
 
 
 section InterleaveAt
