Nemonuri/TransitionSystemLike/ProgramGraph/Interleaving.lean
@@ -19,63 +19,206 @@ open HasHUnion
 
 namespace EvalLike
 
-universe uvar_l uval_l uec uvar_r uval_r uec_r
+universe uvar_l uval_l uec_l uvar_r uval_r uec_r
 
 structure IsInterleaving
-  (VarL1 VarL2: Type uvar_l) (ValL1 ValL2: Type uval_l) (EC1 EC2: Type uec) [EvalLike EC1 VarL1 ValL1] [EvalLike EC2 VarL2 ValL2]
-  (VarR: Type uvar_r) (ValR: Type uval_r) [HasHUnion VarL1 VarL2 VarR] [HasHUnion ValL1 ValL2 ValR]
-  (op: EC1 → EC2 → (HUnionElemAt VarL1 VarL2 VarR) → (HUnionElemAt ValL1 ValL2 ValR)) : Prop where
-  diff_fst (x: HDiffElemAt VarL1 VarL2 VarR .fst) (ec1: EC1) (ec2: EC2) :
+  (VarL1 VarL2: Type uvar_l) (ValL1 ValL2: Type uval_l) (EC1 EC2: Type uec_l) [EvalLike EC1 VarL1 ValL1] [EvalLike EC2 VarL2 ValL2]
+  [HasHUnion VarL1 VarL2] [HasHUnion ValL1 ValL2]
+  (op: EC1 → EC2 → (HUnionElemAt VarL1 VarL2) → (HUnionElemAt ValL1 ValL2)) : Prop where
+  diff_fst (x: HDiffElemAt VarL1 VarL2 .fst) (ec1: EC1) (ec2: EC2) :
     .ofEmbedElem (EmbedElemAt.mapAt VarL1 VarL2 ValL1 ValL2 .fst (ec1: Eval VarL1 ValL1) x.toEmbedElem) = op ec1 ec2 (.ofEmbedElem x.toEmbedElem)
-  diff_snd (x: HDiffElemAt VarL1 VarL2 VarR .snd) (ec1: EC1) (ec2: EC2) :
+  diff_snd (x: HDiffElemAt VarL1 VarL2 .snd) (ec1: EC1) (ec2: EC2) :
     .ofEmbedElem (EmbedElemAt.mapAt VarL1 VarL2 ValL1 ValL2 .snd (ec2: Eval VarL2 ValL2) x.toEmbedElem) = op ec1 ec2 (.ofEmbedElem x.toEmbedElem)
-  inter (x: HInterElemAt VarL1 VarL2 VarR) (ec1: EC1) (ec2: EC2) :
+  inter (x: HInterElemAt VarL1 VarL2) (ec1: EC1) (ec2: EC2) :
     let rhs := op ec1 ec2 (x.toUnion)
     (.ofEmbedElem (EmbedElemAt.mapAt VarL1 VarL2 ValL1 ValL2 .fst (ec1: Eval VarL1 ValL1) (x.toEmbedElemAt .fst)) = rhs) ∨
     (.ofEmbedElem (EmbedElemAt.mapAt VarL1 VarL2 ValL1 ValL2 .snd (ec2: Eval VarL2 ValL2) (x.toEmbedElemAt .snd)) = rhs)
 
+structure IsSurjectiveInterleaving
+  (VarL1 VarL2: Type uvar_l) (ValL1 ValL2: Type uval_l) (EC1 EC2: Type uec_l) (ECR: Type uec_r)
+  [HasHUnion VarL1 VarL2] [HasHUnion ValL1 ValL2] [EvalLike EC1 VarL1 ValL1] [EvalLike EC2 VarL2 ValL2] [EvalLike ECR (HUnionElemAt VarL1 VarL2) (HUnionElemAt ValL1 ValL2)]
+  (op: EC1 → EC2 → ECR) : Prop where
+  interleaving: IsInterleaving VarL1 VarL2 ValL1 ValL2 EC1 EC2 (fun ec1 ec2 => op ec1 ec2)
+  surjective: Function.Surjective (Function.uncurry op)
+
+namespace IsSurjectiveInterleaving
+
+variable {VarL1 VarL2: Type uvar_l} {ValL1 ValL2: Type uval_l} {EC1 EC2: Type uec_l} {ECR: Type uec_r}
+         [HasHUnion VarL1 VarL2] [HasHUnion ValL1 ValL2] [EvalLike EC1 VarL1 ValL1] [EvalLike EC2 VarL2 ValL2]
+         [EvalLike ECR (HUnionElemAt VarL1 VarL2) (HUnionElemAt ValL1 ValL2)]
+
+noncomputable def recRightEvalCarrier
+  {op: EC1 → EC2 → ECR} (h: IsSurjectiveInterleaving VarL1 VarL2 ValL1 ValL2 EC1 EC2 ECR op)
+  {motive: ECR → Sort _}
+  (left: (ec1: EC1) → (ec2: EC2) → motive (op ec1 ec2))
+  (t: ECR)
+  : motive t :=
+  match lm1: Classical.choose (h.surjective t) with
+  | ⟨ec1, ec2⟩ => left ec1 ec2 |> Eq.subst (by
+      have lm2 := Classical.choose_spec (h.surjective t)
+      rewrite [lm1] at lm2
+      simpa using lm2 )
+
+end IsSurjectiveInterleaving
+
 
 structure Interleaving
-  (VarL1 VarL2: Type uvar_l) (ValL1 ValL2: Type uval_l) (EC1 EC2: Type uec) [EvalLike EC1 VarL1 ValL1] [EvalLike EC2 VarL2 ValL2]
-  (VarR: Type uvar_r) (ValR: Type uval_r) [HasHUnion VarL1 VarL2 VarR] [HasHUnion ValL1 ValL2 ValR] where
-  op (ec1: EC1) (ec2: EC2) : (HUnionElemAt VarL1 VarL2 VarR) → (HUnionElemAt ValL1 ValL2 ValR)
-  valid: IsInterleaving VarL1 VarL2 ValL1 ValL2 EC1 EC2 VarR ValR op
+  (VarL1 VarL2: Type uvar_l) (ValL1 ValL2: Type uval_l) (EC1 EC2: Type uec_l) (ECR: Type uec_r)
+  [HasHUnion VarL1 VarL2] [HasHUnion ValL1 ValL2] [EvalLike EC1 VarL1 ValL1] [EvalLike EC2 VarL2 ValL2]
+  [EvalLike ECR (HUnionElemAt VarL1 VarL2) (HUnionElemAt ValL1 ValL2)] where
+  op (ec1: EC1) (ec2: EC2) : ECR
+  valid: IsSurjectiveInterleaving VarL1 VarL2 ValL1 ValL2 EC1 EC2 ECR op
+  --op_interleaving: IsInterleaving VarL1 VarL2 ValL1 ValL2 EC1 EC2 (fun ec1 ec2 => op ec1 ec2)
+  --op_surjective: Function.Surjective (Function.uncurry op)
+
 
 
 namespace Interleaving
 
-variable {VarL1 VarL2: Type uvar_l} {ValL1 ValL2: Type uval_l} {EC1 EC2: Type uec} [EvalLike EC1 VarL1 ValL1] [EvalLike EC2 VarL2 ValL2]
-         {VarR: Type uvar_r} {ValR: Type uval_r} [HasHUnion VarL1 VarL2 VarR] [HasHUnion ValL1 ValL2 ValR]
+variable {VarL1 VarL2: Type uvar_l} {ValL1 ValL2: Type uval_l} {EC1 EC2: Type uec_l} {ECR: Type uec_r}
+         [HasHUnion VarL1 VarL2] [HasHUnion ValL1 ValL2] [EvalLike EC1 VarL1 ValL1] [EvalLike EC2 VarL2 ValL2]
+         [EvalLike ECR (HUnionElemAt VarL1 VarL2) (HUnionElemAt ValL1 ValL2)]
 
 
-theorem op_injective : Function.Injective (@op VarL1 VarL2 ValL1 ValL2 EC1 EC2 _ _ VarR ValR _ _) := by
+
+theorem op_injective : Function.Injective (@op VarL1 VarL2 ValL1 ValL2 EC1 EC2 ECR _ _ _ _ _) := by
   rintro ⟨te1, lm1⟩ ⟨te2, lm2⟩ lm3
   simp at lm3 ⊢
   exact lm3
 
-
-structure Eval (il: Interleaving VarL1 VarL2 ValL1 ValL2 EC1 EC2 VarR ValR) (ec1: EC1) (ec2: EC2) where
-  eval: (HUnionElemAt VarL1 VarL2 VarR) → (HUnionElemAt ValL1 ValL2 ValR)
+/-
+structure Eval (il: Interleaving VarL1 VarL2 ValL1 ValL2 EC1 EC2) (ec1: EC1) (ec2: EC2) where
+  eval: (HUnionElemAt VarL1 VarL2) → (HUnionElemAt ValL1 ValL2)
   valid: eval = il.op ec1 ec2
 
-def toEval (ec1: EC1) (ec2: EC2) (il: Interleaving VarL1 VarL2 ValL1 ValL2 EC1 EC2 VarR ValR) : Eval il ec1 ec2 where
+def toEval (ec1: EC1) (ec2: EC2) (il: Interleaving VarL1 VarL2 ValL1 ValL2 EC1 EC2) : Eval il ec1 ec2 where
   eval := il.op ec1 ec2
   valid := rfl
 
-instance {il: Interleaving VarL1 VarL2 ValL1 ValL2 EC1 EC2 VarR ValR} {ec1: EC1} {ec2: EC2} : EvalLike (Eval il ec1 ec2) (HUnionElemAt VarL1 VarL2 VarR) (HUnionElemAt ValL1 ValL2 ValR) where
+instance {il: Interleaving VarL1 VarL2 ValL1 ValL2 EC1 EC2} {ec1: EC1} {ec2: EC2} : EvalLike (Eval il ec1 ec2) (HUnionElemAt VarL1 VarL2) (HUnionElemAt ValL1 ValL2) where
   coe x := .mk x.eval
   coe_injective := by rintro ⟨_,_⟩ ⟨_,_⟩; simp
+-/
 
 end Interleaving
+
+class HasInterleaving (EC1 EC2: Type uec_l) (Var1 Var2: Type uvar_l) (Val1 Val2: Type uval_l) [EvalLike EC1 Var1 Val1] [EvalLike EC2 Var2 Val2] where
+  var: HasHUnion.Bundle.{uvar_l, uvar_r} Var1 Var2
+  val: HasHUnion.Bundle.{uval_l, uval_r} Val1 Val2
+  R: Type uec_r
+  evalLikeR: EvalLike R (HUnionElemAt Var1 Var2) (HUnionElemAt Val1 Val2)
+  interleaving: Interleaving Var1 Var2 Val1 Val2 EC1 EC2 R
+
+attribute [reducible, instance] HasInterleaving.var HasInterleaving.val HasInterleaving.evalLikeR
 
 end EvalLike
 
 
---structure Interleaving
+namespace StandardType
 
---namespace Interleaving
+open EvalLike
 
---end Interleaving
+variable {EC1 EC2: Type uec_l} {Var1 Var2: Type uvar_l} {Val1 Val2: Type uval_l} [EvalLike EC1 Var1 Val1] [EvalLike EC2 Var2 Val2]
+         [HasInterleaving EC1 EC2 Var1 Var2 Val1 Val2]
+
+def SetOfInterleavingValueDomainAt (sty1: StandardType EC1 Var1 Val1) (sty2: StandardType EC2 Var2 Val2) (var: HUnionElemAt Var1 Var2) : Set (HUnionElemAt Val1 Val2) :=
+  let s1 : Set Val1 := var.recLiftDiffAt .fst (fun x => sty1.dom x.liftAt) (fun _ => ∅)
+  let s2 : Set Val2 := var.recLiftDiffAt .snd (fun x => sty2.dom x.liftAt) (fun _ => ∅)
+  HUnionElemAt.setOfHUnion s1 s2
+
+
+def interleave (sty1: StandardType EC1 Var1 Val1) (sty2: StandardType EC2 Var2 Val2) : StandardType (HasInterleaving.R EC1 EC2 Var1 Var2 Val1 Val2) (HUnionElemAt Var1 Var2) (HUnionElemAt Val1 Val2) where
+  dom := SetOfInterleavingValueDomainAt sty1 sty2
+  valid ec var := by
+    have lm1 := sty1.valid
+    have lm2 := sty2.valid
+    let il : Interleaving Var1 Var2 Val1 Val2 EC1 EC2 _ := HasInterleaving.interleaving
+    rcases il with ⟨op, lm3⟩
+    cases ec using (IsSurjectiveInterleaving.recRightEvalCarrier lm3)
+    rename_i ec1 ec2
+    specialize lm1 ec1
+    specialize lm2 ec2
+    cases var using HUnionElemAt.recDiffInter <;> rename_i x
+    · let x2 := x.toEmbedElem
+      specialize lm1 x2.liftAt
+      dsimp [SetOfInterleavingValueDomainAt, HUnionElemAt.setOfHUnion]
+      refine Or.inl ?_
+      simp
+      exists ((ec1: Eval Var1 Val1) x2.liftAt)
+      refine ⟨?_, ?_⟩
+      · simp [HUnionElemAt.recLiftDiffAt, DecidableEmbedRange.isInEmbedRangeAt_eq_true_iff, HUnionElemAt.ofEmbedElem]
+        exact lm1
+      · subst x2
+        rcases lm3 with ⟨⟨lm3_1, lm3_2, lm3_3⟩, lm3_4⟩
+        specialize lm3_1 x ec1 ec2
+        exact lm3_1
+    · let x2 := x.toEmbedElem
+      specialize lm2 x2.liftAt
+      dsimp [SetOfInterleavingValueDomainAt, HUnionElemAt.setOfHUnion]
+      refine Or.inr ?_
+      simp
+      exists ((ec2: Eval Var2 Val2) x2.liftAt)
+      refine ⟨?_, ?_⟩
+      · simp [HUnionElemAt.recLiftDiffAt, DecidableEmbedRange.isInEmbedRangeAt_eq_true_iff, HUnionElemAt.ofEmbedElem]
+        exact lm2
+      · subst x2
+        rcases lm3 with ⟨⟨lm3_1, lm3_2, lm3_3⟩, lm3_4⟩
+        specialize lm3_2 x ec1 ec2
+        exact lm3_2
+    · rcases lm3 with ⟨⟨lm3_1, lm3_2, lm3_3⟩, lm3_4⟩
+      clear lm3_1 lm3_2 lm3_4
+      specialize lm3_3 x ec1 ec2
+      dsimp at lm3_3
+      let x1 := x.toEmbedElemAt .fst
+      let x2 := x.toEmbedElemAt .snd
+      specialize lm1 x1.liftAt
+      specialize lm2 x2.liftAt
+      rcases lm3_3 with lm3_3 | lm3_3
+      · rw [← lm3_3]
+        dsimp [SetOfInterleavingValueDomainAt, HUnionElemAt.setOfHUnion]
+        simp
+        refine Or.inl ?_
+        exists ((ec1: Eval Var1 Val1) x1.liftAt)
+        refine ⟨?_, ?_⟩
+        · have lm4 := x.property
+          rewrite [hinterSetUnivAt_mem_iff_isInEmbedRangeAt] at lm4
+          replace lm4 := lm4.left
+          simp [HUnionElemAt.recLiftDiffAt, HInterElemAt.toUnion, lm4]
+          subst x1
+          conv at lm1 =>
+            arg 1
+            dsimp [HInterElemAt.toEmbedElemAt, EmbedElemAt.pureAt, HInterElemAt.liftAt]
+            simp [liftAt_embedAt_eq]
+          exact lm1
+        · subst x1
+          dsimp [HInterElemAt.toEmbedElemAt, HInterElemAt.liftAt, EmbedElemAt.pureAt, EmbedElemAt.liftAt]
+          simp [liftAt_embedAt_eq]
+          dsimp [EmbedElemAt.mapAt, EmbedElemAt.bindAt, EmbedElemAt.pureAt, EmbedElemAt.liftAt]
+      · rw [← lm3_3]
+        dsimp [SetOfInterleavingValueDomainAt, HUnionElemAt.setOfHUnion]
+        simp
+        refine Or.inr ?_
+        exists ((ec2: Eval Var2 Val2) x2.liftAt)
+        refine ⟨?_, ?_⟩
+        · have lm4 := x.property
+          rewrite [hinterSetUnivAt_mem_iff_isInEmbedRangeAt] at lm4
+          replace lm4 := lm4.right
+          simp [HUnionElemAt.recLiftDiffAt, HInterElemAt.toUnion, lm4]
+          subst x2
+          conv at lm2 =>
+            arg 1
+            dsimp [HInterElemAt.toEmbedElemAt, EmbedElemAt.pureAt, HInterElemAt.liftAt]
+            simp [liftAt_embedAt_eq]
+          exact lm2
+        · subst x2
+          dsimp [HInterElemAt.toEmbedElemAt, HInterElemAt.liftAt, EmbedElemAt.pureAt, EmbedElemAt.liftAt]
+          simp [liftAt_embedAt_eq]
+          dsimp [EmbedElemAt.mapAt, EmbedElemAt.bindAt, EmbedElemAt.pureAt, EmbedElemAt.liftAt]
+
+
+
+end StandardType
+
 
 end Nemonuri.ProgramGraph
 
